src/syntax.lean
@@ -3,8 +3,6 @@
 import data.fintype data.finmap data.bool data.vector data.list
 import util
 
-variable {α : Type}
-
 /- Each program has names. Names consist of a finite set of class names, a finite set of record names, and a finite set of symbol names. To each class name, there an associated finite set of field and method names. There is a built-in record name, boolean. -/
 class names (α : Type) :=
   (decidable_name: decidable_eq α)
@@ -15,7 +13,7 @@ class names (α : Type) :=
   (Nm {x : α} (H: x ∈ Nc): finset α)
   (Nboolean : α)
   (Hboolean : Nboolean ∈ Nr)
-instance names.decidable [names α]:
+instance names.decidable {α : Type} [names α]:
   decidable_eq α := names.decidable_name α
 
 /- We make use of subtypes, to demonstrate instances of fintype. Whenever we have established that these types are finite, we obtain decidable equality for functions that take these types as domain (thanks to Johannes Hölzl). This fact turns out to be crucial for semantics. -/
@@ -32,10 +30,10 @@ def symbol_name (α : Type) [names α] :=
 def boolean_name (α : Type) [names α] : record_name α :=
   ⟨names.Nboolean α, names.Hboolean α⟩
 @[reducible]
-def field_name [names α] (self : class_name α) :=
+def field_name {α : Type} [names α] (self : class_name α) :=
   {name : α // name ∈ names.Nf self.property}
 @[reducible]
-def method_name [names α] (self : class_name α) :=
+def method_name {α : Type} [names α] (self : class_name α) :=
   {name : α // name ∈ names.Nm self.property}
 
 /- A type in our object language is either: a reference type (by class name), or a data type (by record name). -/
@@ -51,14 +49,14 @@ inductive type (α : Type) [names α]
   (type.data (boolean_name α))
 
 /- A class declaration (of some class self) consists of a map from field names to field declarations, a map from method names to method declarations, and a method name that indicates a constructor. A field declaration consists of a type. A method declaration consists of a map from parameter names to parameter declarations. A parameter declaration consists of a type. -/
-structure mdecl [names α]
+structure mdecl {α : Type} [names α]
     {self : class_name α} (m : method_name self) :=
   (args : list (type α))
-structure fdecl [names α]
+structure fdecl {α : Type} [names α]
     {self : class_name α} (f : field_name self) :=
   (type : type α)
 -- Design choice: constructors and methods are treated uniformly.
-structure cdecl [names α] (self : class_name α) :=
+structure cdecl {α : Type} [names α] (self : class_name α) :=
   (fdecl (f : field_name self) : fdecl f)
   (mdecl (m : method_name self) : mdecl m)
   (ctor : method_name self)
@@ -76,60 +74,66 @@ class signature (α : Type) extends names α :=
   (sdef (x : symbol_name α) : sdecl α)
   (main: class_name α)
 
-variable [signature α]
-variable {self : class_name α}
-
 /- Each parameter is associated to a type, each field is associated to a type, and each class name is associated to a constructor method name. -/
-def param_types (m : method_name self) : list (type α) :=
+def param_types {α : Type} [signature α] {self : class_name α}
+    (m : method_name self) : list (type α) :=
   ((signature.cdef self).mdecl m).args
-def field_type (f : field_name self) : type α :=
+def field_type {α : Type} [signature α] {self : class_name α}
+    (f : field_name self) : type α :=
   ((signature.cdef self).fdecl f).type
-def ctor (self : class_name α) : method_name self :=
+def ctor {α : Type} [signature α] (self : class_name α) :
+    method_name self :=
   (signature.cdef self).ctor
 /- A symbol with zero arity is a constant symbol, a symbol with non-zero arity is a function symbol. Each symbol is associated to a result type. A function symbol is associated to a list of argument types. -/
 @[derive decidable_eq]
-structure symbol (args : list (type α)) (result : type α)
+structure symbol {α : Type} [signature α]
+    (args : list (type α)) (result : type α)
     (s : symbol_name α) :=
   (H: args = (signature.sdef s).args)
   (G: result = (signature.sdef s).result)
-def symbol.name {args : list (type α)} {result : type α}
-    {s : symbol_name α} (sym : symbol args result s) := s
+def symbol.name {α : Type} [signature α]
+  {args : list (type α)} {result : type α}
+  {s : symbol_name α} (sym : symbol args result s) := s
 
 /- Given a signature and an enclosing class, we consider type environments to consist of: a method name, and declared local variables. -/
 @[derive decidable_eq]
-structure tenv (self : class_name α) :=
+structure tenv {α : Type} [signature α] (self : class_name α) :=
   (current : method_name self)
   (locals : context α)
-def tenv.self (e : tenv self) : class_name α :=
-  self
-def tenv.args (e : tenv self) : list (type α) :=
-  param_types e.current
+def tenv.self {α : Type} [signature α] {self : class_name α}
+  (e : tenv self) : class_name α := self
+def tenv.args {α : Type} [signature α] {self : class_name α}
+  (e : tenv self) : list (type α) := param_types e.current
 
 /- A note on terminology. Parameter: as declared in signature. Argument: a pure expression as supplied in a method call, or as supplied to a function symbol. -/
 
 /- Within a typing environment, we refer to numerous things. This refers to an object identity of the enclosed class. A local variable refers to the index within the declared local variables. A parameter refers to a parameter name of the current method. A field refers to a field within the enclosed class. -/
-section
-variables (e : tenv self) (ty : type α)
 @[derive decidable_eq]
-structure tvar :=
+structure tvar {α : Type} [signature α] {self : class_name α}
+    (e : tenv self) (ty : type α) :=
   (H : ty = type.ref e.self)
 @[derive decidable_eq]
-structure lvar :=
+structure lvar {α : Type} [signature α] {self : class_name α}
+    (e : tenv self) (ty : type α):=
   (idx : list_at ty e.locals)
 @[derive decidable_eq]
-structure pvar :=
+structure pvar {α : Type} [signature α] {self : class_name α}
+    (e : tenv self) (ty : type α) :=
   (idx : list_at ty e.args)
 @[derive decidable_eq]
-structure fvar :=
+structure fvar {α : Type} [signature α] {self : class_name α}
+    (e : tenv self) (ty : type α) :=
   (idx : field_name e.self) (H : field_type idx = ty)
 -- Store variable (LHS only)
 @[derive decidable_eq]
-inductive svar
+inductive svar {α : Type} [signature α] {self : class_name α}
+    (e : tenv self) (ty : type α)
 | fvar: fvar e ty → svar
 | lvar: lvar e ty → svar
 -- Read variable (RHS only)
 @[derive decidable_eq]
-inductive rvar
+inductive rvar {α : Type} [signature α] {self : class_name α}
+    (e : tenv self) (ty : type α)
 | tvar: tvar e ty → rvar
 | fvar: fvar e ty → rvar
 | pvar: pvar e ty → rvar
@@ -139,7 +143,8 @@ end
 /- A pure expression within a typing environment is either: a constant, a function application, value lookup in environment, 
 equality check. -/
 @[derive decidable_eq]
-inductive pexp (e : tenv self) : list (type α) → Type
+inductive pexp {α : Type} [signature α] {self : class_name α}
+    (e : tenv self) : list (type α) → Type
 | const {ty : type α} {c : symbol_name α}:
     symbol [] ty c → pexp [ty]
 | app {l : list (type α)} {ty : type α} {f : symbol_name α}:
@@ -151,7 +156,8 @@ inductive pexp (e : tenv self) : list (type α) → Type
 | cons {ty : type α} {l : list (type α)}:
     pexp [ty] → pexp l → pexp (ty::l)
 /- The encoding of a mutual inductive type fails in Lean 3.4.2. We currently encode this directly, by considering single expressions as expressions with a length one type list. Tuples of expressions are created by constructing lists of expressions of length one lists of types. There are no expressions of empty lists of types. -/
-lemma pexp_not_nil {e : tenv self} {l : list (type α)}
+lemma pexp_not_nil {α : Type} [signature α]
+  {self : class_name α} {e : tenv self} {l : list (type α)}
   (p : pexp e l) : l ≠ [] :=
 begin
   cases l, {intro, cases p}, {intro, cases a}
@@ -159,7 +165,8 @@ end
 
 /- A statement within a typing environment is either: a skip, a sequential composition, a branch, a loop, an assignment, an asynchronous method call, an object allocation. -/
 @[derive decidable_eq]
-inductive stmt (e : tenv self) : bool → Type
+inductive stmt {α : Type} [signature α] {self : class_name α}
+    (e : tenv self) : bool → Type
 | ite: pexp e [boolean α] → stmt tt → stmt tt → stmt ff
 | while: pexp e [boolean α] → stmt tt → stmt ff
 | assign {ty : type α} (l : svar e ty):
@@ -175,20 +182,26 @@ inductive stmt (e : tenv self) : bool → Type
 | cons: stmt ff → stmt tt → stmt tt
 /- The encoding of a nested inductive type failed at the moment in Lean 3.4.2. Instead, we encode the nesting ourselves: the boolean argument determines which constructors are applicable. It is true if it is a list of statements, false if it is a single statement (thanks to Mario Carneiro).  -/
 @[reducible]
-def statement (e : tenv self) := stmt e ff
-variable {e : tenv self}
-def stmt.from_list : list (statement e) → stmt e tt
+def statement {α : Type} [signature α] {self : class_name α}
+  (e : tenv self) := stmt e ff
+def stmt.from_list {α : Type} [signature α]
+    {self : class_name α} {e : tenv self} :
+    list (statement e) → stmt e tt
 | [] := stmt.nil e
 | (x :: xs) := stmt.cons x (stmt.from_list xs)
-def stmt.to_list : stmt e tt → list (statement e)
+def stmt.to_list {α : Type} [signature α]
+    {self : class_name α} {e : tenv self} :
+    stmt e tt → list (statement e)
 | (stmt.nil .(e)) := []
 | (stmt.cons x xs) := (x :: stmt.to_list xs)
 
 /- A program with a given program signature associates to each method of each class a program block. A program block associated to a method consists of: local variable declarations, and a statement within a typing environment. -/
-structure pblock (m : method_name self) :=
+structure pblock {α : Type} [signature α]
+    {self : class_name α} (m : method_name self) :=
   (locals : context α)
   (S : list (statement ⟨m,locals⟩))
-def pblock.tenv {m : method_name self} (pb : pblock m) :=
+def pblock.tenv {α : Type} [signature α] {self : class_name α}
+    {m : method_name self} (pb : pblock m) :=
   (tenv.mk m pb.locals)
 structure program (α : Type) [signature α] :=
   (body {self : class_name α} (m : method_name self): pblock m)
